Switch to a more precise version of interp_related for rewrites
This version is hopefully the right one.  It seems to be basically
exactly what we want to say, and no more and no less.  The rule for
let-ins, which is almost the only freedom we have here, is chosen to
match exactly with the rule for App+Abs.  Note that using Leibniz
equality is essential in the places where it's used.  The recursive
relation here might actually be a bit clearer as an inductive relation,
but I wanted it to simplify under reduction.

After     | File Name                                                            | Before    || Change    | % Change
--------------------------------------------------------------------------------------------------------------------
30m04.79s | Total                                                                | 29m51.25s || +0m13.54s | +0.75%
--------------------------------------------------------------------------------------------------------------------
1m53.11s  | Experiments/NewPipeline/RewriterRulesInterpGood.vo                   | 1m35.74s  || +0m17.36s | +18.14%
0m19.40s  | Experiments/NewPipeline/RewriterWf1.vo                               | 0m24.54s  || -0m05.14s | -20.94%
6m13.78s  | Experiments/NewPipeline/SlowPrimeSynthesisExamples.vo                | 6m14.86s  || -0m01.08s | -0.28%
4m39.23s  | Experiments/NewPipeline/Toplevel1.vo                                 | 4m38.21s  || +0m01.02s | +0.36%
1m31.62s  | Experiments/NewPipeline/Toplevel2.vo                                 | 1m32.68s  || -0m01.06s | -1.14%
0m40.01s  | Experiments/NewPipeline/AbstractInterpretationWf.vo                  | 0m38.77s  || +0m01.23s | +3.19%
3m19.74s  | p384_32.c                                                            | 3m19.71s  || +0m00.03s | +0.01%
1m58.86s  | Experiments/NewPipeline/RewriterWf2.vo                               | 1m58.30s  || +0m00.56s | +0.47%
1m02.04s  | Experiments/NewPipeline/RewriterRulesGood.vo                         | 1m02.41s  || -0m00.36s | -0.59%
0m40.71s  | p521_32.c                                                            | 0m40.51s  || +0m00.20s | +0.49%
0m39.90s  | Experiments/NewPipeline/ExtractionHaskell/word_by_word_montgomery    | 0m39.85s  || +0m00.04s | +0.12%
0m36.76s  | Experiments/NewPipeline/Rewriter.vo                                  | 0m36.81s  || -0m00.05s | -0.13%
0m35.34s  | Experiments/NewPipeline/LanguageInversion.vo                         | 0m35.16s  || +0m00.18s | +0.51%
0m33.80s  | p521_64.c                                                            | 0m33.82s  || -0m00.02s | -0.05%
0m28.97s  | Experiments/NewPipeline/GENERATEDIdentifiersWithoutTypesProofs.vo    | 0m29.54s  || -0m00.57s | -1.92%
0m27.65s  | Experiments/NewPipeline/LanguageWf.vo                                | 0m28.11s  || -0m00.46s | -1.63%
0m25.94s  | Experiments/NewPipeline/ExtractionHaskell/unsaturated_solinas        | 0m25.39s  || +0m00.55s | +2.16%
0m25.63s  | Experiments/NewPipeline/UnderLetsProofs.vo                           | 0m25.15s  || +0m00.48s | +1.90%
0m22.84s  | Experiments/NewPipeline/AbstractInterpretationZRangeProofs.vo        | 0m23.11s  || -0m00.26s | -1.16%
0m18.51s  | Experiments/NewPipeline/ExtractionHaskell/saturated_solinas          | 0m18.69s  || -0m00.17s | -0.96%
0m17.42s  | Experiments/NewPipeline/AbstractInterpretationProofs.vo              | 0m17.29s  || +0m00.13s | +0.75%
0m15.12s  | Experiments/NewPipeline/ExtractionOCaml/word_by_word_montgomery      | 0m14.96s  || +0m00.15s | +1.06%
0m14.43s  | secp256k1_32.c                                                       | 0m14.22s  || +0m00.20s | +1.47%
0m14.19s  | p256_32.c                                                            | 0m14.46s  || -0m00.27s | -1.86%
0m12.72s  | Experiments/NewPipeline/CStringification.vo                          | 0m12.80s  || -0m00.08s | -0.62%
0m10.88s  | p384_64.c                                                            | 0m10.99s  || -0m00.10s | -1.00%
0m09.16s  | Experiments/NewPipeline/ExtractionOCaml/unsaturated_solinas          | 0m08.87s  || +0m00.29s | +3.26%
0m09.14s  | Experiments/NewPipeline/ExtractionOCaml/word_by_word_montgomery.ml   | 0m09.33s  || -0m00.18s | -2.03%
0m07.96s  | Experiments/NewPipeline/GENERATEDIdentifiersWithoutTypes.vo          | 0m07.96s  || +0m00.00s | +0.00%
0m06.61s  | p224_32.c                                                            | 0m06.52s  || +0m00.09s | +1.38%
0m06.37s  | Experiments/NewPipeline/ExtractionOCaml/unsaturated_solinas.ml       | 0m06.29s  || +0m00.08s | +1.27%
0m05.96s  | Experiments/NewPipeline/ExtractionOCaml/saturated_solinas            | 0m05.60s  || +0m00.36s | +6.42%
0m05.92s  | Experiments/NewPipeline/ExtractionHaskell/word_by_word_montgomery.hs | 0m05.82s  || +0m00.09s | +1.71%
0m04.70s  | Experiments/NewPipeline/ExtractionHaskell/unsaturated_solinas.hs     | 0m04.35s  || +0m00.35s | +8.04%
0m04.50s  | Experiments/NewPipeline/ExtractionOCaml/saturated_solinas.ml         | 0m04.63s  || -0m00.12s | -2.80%
0m03.82s  | Experiments/NewPipeline/ExtractionHaskell/saturated_solinas.hs       | 0m03.62s  || +0m00.19s | +5.52%
0m02.62s  | Experiments/NewPipeline/MiscCompilerPassesProofs.vo                  | 0m02.56s  || +0m00.06s | +2.34%
0m02.31s  | curve25519_32.c                                                      | 0m02.40s  || -0m00.08s | -3.74%
0m02.09s  | secp256k1_64.c                                                       | 0m02.18s  || -0m00.09s | -4.12%
0m02.05s  | p224_64.c                                                            | 0m02.04s  || +0m00.00s | +0.49%
0m01.96s  | p256_64.c                                                            | 0m01.94s  || +0m00.02s | +1.03%
0m01.56s  | curve25519_64.c                                                      | 0m01.54s  || +0m00.02s | +1.29%
0m01.53s  | Experiments/NewPipeline/CLI.vo                                       | 0m01.57s  || -0m00.04s | -2.54%
0m01.26s  | Experiments/NewPipeline/StandaloneHaskellMain.vo                     | 0m01.26s  || +0m00.00s | +0.00%
0m01.22s  | Experiments/NewPipeline/Language.vo                                  | 0m01.26s  || -0m00.04s | -3.17%
0m01.22s  | Experiments/NewPipeline/StandaloneOCamlMain.vo                       | 0m01.21s  || +0m00.01s | +0.82%
0m01.08s  | Experiments/NewPipeline/CompilersTestCases.vo                        | 0m00.99s  || +0m00.09s | +9.09%
0m01.06s  | Experiments/NewPipeline/AbstractInterpretation.vo                    | 0m01.02s  || +0m00.04s | +3.92%
0m00.87s  | Experiments/NewPipeline/RewriterProofs.vo                            | 0m00.97s  || -0m00.09s | -10.30%
0m00.74s  | Experiments/NewPipeline/MiscCompilerPasses.vo                        | 0m00.72s  || +0m00.02s | +2.77%
0m00.48s  | Experiments/NewPipeline/UnderLets.vo                                 | 0m00.52s  || -0m00.04s | -7.69%

src/Experiments/NewPipeline/Language.v
@@ -452,6 +452,39 @@ Module Compilers.
                @interp _ _ _ interp_ident _ (f y)
          end.
 
+    Section with_interp.
+      Context {base_type : Type}
+              {ident : type base_type -> Type}
+              {interp_base_type : base_type -> Type}
+              (interp_ident : forall t, ident t -> type.interp interp_base_type t).
+
+      Fixpoint interp_related {t} (e : @expr base_type ident (type.interp interp_base_type) t) : type.interp interp_base_type t -> Prop
+        := match e in expr t return type.interp interp_base_type t -> Prop with
+           | expr.Var t v1 => fun v2 => v1 == v2
+           | expr.App s d f x
+             => fun v2
+                => exists fv xv,
+                    @interp_related _ f fv
+                    /\ @interp_related _ x xv
+                    /\ fv xv = v2
+           | expr.Ident t idc
+             => fun v2 => interp_ident _ idc == v2
+           | expr.Abs s d f1
+             => fun f2
+                => forall x1 x2,
+                    x1 == x2
+                    -> @interp_related d (f1 x1) (f2 x2)
+           | expr.LetIn s d x f (* combine the App rule with the Abs rule *)
+             => fun v2
+                => exists fv xv,
+                    @interp_related _ x xv
+                    /\ (forall x1 x2,
+                           x1 == x2
+                           -> @interp_related d (f x1) (fv x2))
+                    /\ fv xv = v2
+           end.
+    End with_interp.
+
     Definition Expr {base_type ident} t := forall var, @expr base_type ident var t.
     Definition APP {base_type ident s d} (f : Expr (s -> d)) (x : Expr s) : Expr d
       := fun var => @App base_type ident var s d (f var) (x var).
